improved structure in count and cont.

core/mach/Mmach.v
@@ -15,76 +15,75 @@ Notation "? K" := (@inl (list Q) A' K) (format "'?' K", at level 50).
 Notation "! a'" := (@inr (list Q) A' a') (format "'!' a'", at level 50).
 
 Definition M_step (psi: list A * Q' -> list Q + A') phi q' L :=
-match psi (L, q') with
+  match psi (L, q') with
   | inr a' => inr a'
   | inl K => inl ((map phi K) ++ L)
-end.
+  end.
 
 Fixpoint M_rec (psi: list A * Q' -> list Q + A') n phi q' :=
-match n with
-	|	0 => M_step psi phi q' nil
-	|	S n' => match M_rec psi n' phi q' with
-	  | inr a' => inr a'
-		| inl L => M_step psi phi q' L
-	end
-end.
+  match n with
+  | 0 => M_step psi phi q' nil
+  | S n' => match M_rec psi n' phi q' with
+	   | inr a' => inr a'
+	   | inl L => M_step psi phi q' L
+	   end
+  end.
 
 Definition M
-	(psi: list A * Q' -> list Q + A')
-	(n: nat)
-	(phi: Q -> A)
-	(q' : Q') :=
-match M_rec psi n phi q' with
-	| inr a' => Some a'
-	| inl L => None
-end.
+	   (psi: list A * Q' -> list Q + A')
+	   (n: nat)
+	   (phi: Q -> A)
+	   (q' : Q') :=
+  match M_rec psi n phi q' with
+  | inr a' => Some a'
+  | inl L => None
+  end.
 
-Lemma M_mon psi:
-	(M psi) \is_monotone.
+Lemma M_mon psi: (M psi) \is_monotone.
 Proof. by move => phi phifd q' n; rewrite/M/=; case E: (M_rec psi n phi q'). Qed.
 
 Lemma M_rec_step n psi phi q':
-	M_rec psi n.+1 phi q' = match M_rec psi n phi q' with
-	  | inr a' => inr a'
-		| inl L => M_step psi phi q' L
-	end.
+  M_rec psi n.+1 phi q' = match M_rec psi n phi q' with
+	                  | inr a' => inr a'
+		          | inl L => M_step psi phi q' L
+	                  end.
 Proof. done. Qed.
 
 Lemma M_rec_inl_spec psi n phi q' L:
-	M_rec psi n phi q' =  inl L <-> exists (Ln: list (list A)),
-		size Ln = n.+1 /\ L = flatten Ln /\
-		forall i, i < n.+1 -> exists K,
-			psi (flatten (drop i.+1 Ln), q') = ? K /\
-			flatten (drop i Ln) = map phi K ++ flatten (drop i.+1 Ln).
+  M_rec psi n phi q' =  inl L <-> exists (Ln: list (list A)),
+    size Ln = n.+1 /\ L = flatten Ln /\
+    forall i, i < n.+1 -> exists K,
+	psi (flatten (drop i.+1 Ln), q') = ? K /\
+	flatten (drop i Ln) = map phi K ++ flatten (drop i.+1 Ln).
 Proof.
 split.
-	elim: n L => [L | /= n]; first rewrite /=/M_step.
-		case E: (psi (nil, q')) => [K | ]//; rewrite cats0 => [[]] eq.
-		exists [:: L]; split => //; split => [ | i ineq]; first by rewrite /= cats0.
-		exists K; split => //; have /eqP ->: i == 0 by rewrite -leqn0.
-		by rewrite /= eq.
-	case E: (M_rec psi n phi q') => [L' | ] // ih L /=.
-	have [ | Ln [sze [eq prp E']]]//:= ih L'.
-	move: E'; rewrite /M_step; case val: (psi (L', q')) => [K | ]// [E'].
-	exists (map phi K :: Ln); split => //=; first by rewrite sze.
-	split; first by rewrite -eq E'.
-	case => [_ | i ineq]; last exact/prp.
-	by exists K; rewrite drop0 /=; split; first by rewrite -eq.
+- elim: n L => [L | /= n]; first rewrite /=/M_step.
+  case E: (psi (nil, q')) => [K | ]//; rewrite cats0 => [[]] eq.
+  exists [:: L]; split => //; split => [ | i ineq]; first by rewrite /= cats0.
+  exists K; split => //; have /eqP ->: i == 0 by rewrite -leqn0.
+  by rewrite /= eq.
+case E: (M_rec psi n phi q') => [L' | ] // ih L /=.
+- have [ | Ln [sze [eq prp E']]]//:= ih L'.
+  move: E'; rewrite /M_step; case val: (psi (L', q')) => [K | ]// [E'].
+  exists (map phi K :: Ln); split => //=; first by rewrite sze.
+  split; first by rewrite -eq E'.
+  case => [_ | i ineq]; last exact/prp.
+  by exists K; rewrite drop0 /=; split; first by rewrite -eq.
 elim: n L => [_ [Ln [sze [-> prp]]]/= | /= n ih _ [Ln [sze [-> prp]]]].
-	have [ | K [ ]]//:= prp 0; rewrite drop1 drop0.
-	have -> /=: (behead Ln) = [::] by apply/size0nil; rewrite size_behead sze.
-	by rewrite !cats0 /M_step => -> ->/=; rewrite cats0.
+- have [ | K [ ]]//:= prp 0; rewrite drop1 drop0.
+  have -> /=: (behead Ln) = [::] by apply/size0nil; rewrite size_behead sze.
+  by rewrite !cats0 /M_step => -> ->/=; rewrite cats0.
 rewrite (ih (flatten (drop 1 Ln))); have [ | K [val ]]//:= prp 0.
-	by rewrite drop0 /M_step val => ->.
+  by rewrite drop0 /M_step val => ->.
 move => eq; exists (drop 1 Ln); split; first by rewrite size_drop sze.
 split => // i ineq; have [ | K']//:= prp i.+1 => [[val' eq']].
 by exists K'; split; [rewrite drop_drop -val' addn1 | rewrite !drop_drop !addn1].
 Qed.
 
 Definition consistent (psi: _ -> _ + A') (phi: B) (q': Q') Ln := forall i, i < size Ln -> exists K,
-			psi (flatten (drop i.+1 Ln), q') = ? K
-			/\
-			flatten (drop i Ln) = map phi K ++ flatten (drop i.+1 Ln).
+      psi (flatten (drop i.+1 Ln), q') = ? K
+      /\
+      flatten (drop i Ln) = map phi K ++ flatten (drop i.+1 Ln).
 
 Lemma cns0 psi phi q': consistent psi phi q' nil.
 Proof. done. Qed.
@@ -128,9 +127,9 @@ Lemma cns_rec psi phi q' Ln Ln' a': psi (flatten Ln, q') = ! a' -> size Ln <= si
 	consistent psi phi q' Ln -> consistent psi phi q' Ln' -> Ln = Ln'.
 Proof.
 move => val; elim: Ln' => [ | L' Ln' ih].
-	by rewrite leqn0 => /eqP eq; rewrite (size0nil eq).
+  by rewrite leqn0 => /eqP eq; rewrite (size0nil eq).
 rewrite leq_eqVlt; case /orP => [/eqP eq | ineq cns cns'].
-	by case: Ln eq ih val => // L Ln eq ih val cns cns'; exact/cns_eq/cns'/cns.
+  by case: Ln eq ih val => // L Ln eq ih val cns cns'; exact/cns_eq/cns'/cns.
 have [ | K [/=]]//:= cns' 0.
 have <-: Ln = Ln' by apply/ih => // i ineq'; apply cns'.
 by rewrite drop0 val.
@@ -143,7 +142,7 @@ Lemma cmcn_unique psi phi: (communication psi phi) \is_singlevalued.
 Proof.
 move => q' [Ln a'] [Ln' b'] [/=cns val] [cns' val'].
 case/orP: (leq_total (size Ln) (size Ln')) => ineq.
-	by move: val'; have <-:= cns_rec val ineq cns cns'; rewrite val => [[->]].
+  by move: val'; have <-:= cns_rec val ineq cns cns'; rewrite val => [[->]].
 by move: val; have <-:= cns_rec val' ineq cns' cns; rewrite val' => [[->]].
 Qed.
 
@@ -158,13 +157,13 @@ Lemma FM_val_spec psi phi Fphi: \F_(M psi) phi Fphi <->
 	forall q', exists (Ln: list (list A)), communication psi phi q' (Ln, (Fphi q')).
 Proof.
 split => val q'.
-	have [n]:= val q'.
-	elim: n => [ | n ih /=]; rewrite /M/=/M_step.
-		by case E: (psi (nil, q')) => [ | a']// [eq]; exists nil; rewrite E eq; split.
-	case E: (M_rec psi n phi q') => [L | a']; last by move => eq; apply/ih; rewrite /M /= E eq.
-	case E': (psi (L, q')) => [ | a']// [eq].
-	have [Ln [<- [eq' prp]]]:= (M_rec_inl_spec psi n phi q' L).1 E.
-	by exists Ln; split; last by rewrite -eq' E' eq.
+- have [n]:= val q'.
+  elim: n => [ | n ih /=]; rewrite /M/=/M_step.
+    by case E: (psi (nil, q')) => [ | a']// [eq]; exists nil; rewrite E eq; split.
+  case E: (M_rec psi n phi q') => [L | a']; last by move => eq; apply/ih; rewrite /M /= E eq.
+  case E': (psi (L, q')) => [ | a']// [eq].
+  have [Ln [<- [eq' prp]]]:= (M_rec_inl_spec psi n phi q' L).1 E.
+  by exists Ln; split; last by rewrite -eq' E' eq.
 have [Ln [eq prp]]:= val q'.
 elim: Ln eq prp => [_ /= eq | L Ln ih prp eq/=]; first by exists 0; rewrite/M/=/M_step eq.
 exists (size Ln).+1; rewrite /M/=/M_step.
@@ -174,7 +173,6 @@ Qed.
 
 Definition mf_dialogue psi phi := make_mf (fun q' a =>
 	exists Ln, consistent psi phi q' Ln /\ List.In a (flatten Ln)).
-
 
 Lemma dlg_com psi phi q' a: mf_dialogue psi phi q' a -> 
 	forall Ln a', communication psi phi q' (Ln, a') -> List.In a (flatten Ln).
@@ -218,7 +216,7 @@ Lemma queries psi phi: phi*)
 End universal_machine.
 
 Section psiF.
-Context (Q Q' A A': Type) (noq: Q).
+Context (Q Q' A A': Type).
 Notation B := (Q -> A).
 Notation B' := (Q' -> A').
 Context (cnt: nat -> Q).
@@ -228,25 +226,24 @@ Context (listf: seq A -> B).
 Context (mf: B -> Q' -> nat).
 Context (FF: B -> B').
 
-Definition psiF (Lq': seq A * Q') := let phi:= listf Lq'.1 in let n:= size Lq'.1 in let q' := Lq'.2 in
+Definition psiF (Lq': seq A * Q') :=
+  let phi:= listf Lq'.1 in let n:= size Lq'.1 in let q' := Lq'.2 in
 	if mf phi q' <= n then inr (FF phi q') else (inl (segment n (mf phi q').-1)).
 
 Lemma psiF_size n phi q' L: M_rec psiF n phi q' = inl L -> n < size L.
 Proof.
 elim: n L => [L | n ih L /=].
-	by rewrite /psiF/=/M_step/=; case E: (mf (listf nil) q') => [ | m /=]; last by move => [<-].
+  by rewrite /psiF/=/M_step/=; case E: (mf (listf nil) q') => [ | m /=]; last by move => [<-].
 case E: (M_rec psiF n phi q') => [K | ]//.
 rewrite /M_step/psiF /=.
 case E': (mf (listf K) q' <= size K) => //.
-move => [<-].
-case eq': (mf (listf K) q') E' => [ | k] //= E'.
+move => [<-]; case eq': (mf (listf K) q') E' => [ | k] //= E'.
 rewrite size_cat size_map size_seg subnK; last by rewrite leqW // leqNgt E'.
 apply/leq_trans; first by have ineq': n.+1 < (size K).+1; [apply/ih | apply/ineq'].
 by rewrite ltnNge E'.
 Qed.
 
-Lemma psiF_spec phi q':
-	forall n,
+Lemma psiF_spec phi q' n:
 		(exists k,
 		mf (listf (map phi (init_seg k))) q' <= k
 		/\
@@ -255,25 +252,23 @@ Lemma psiF_spec phi q':
 	forall m, m <= n -> exists k, M_rec psiF m phi q' = inl (map phi (init_seg k)).
 Proof.
 pose phin m := listf (map phi (init_seg m)).
-elim => [ | n ih].
-	rewrite /M_rec/M_step/psiF/=.
-	case E: (mf (listf [::]) q' <= 0); first by left; exists 0; split.
-	right => m; rewrite leqn0 => /eqP ->; rewrite E /=.
-	by case S: (mf (listf nil) q') E => [ | n]// _; exists n.+1; rewrite cats0 iseg_seg.
+elim: n => [ | n ih].
+- rewrite /M_rec/M_step/psiF/=.
+  case E: (mf (listf [::]) q' <= 0); first by left; exists 0; split.
+  right => m; rewrite leqn0 => /eqP ->; rewrite E /=.
+  by case S: (mf (listf nil) q') E => [ | n]// _; exists n.+1; rewrite cats0 iseg_seg.
 case: ih => [[] m [] ineq | prp].
-	by rewrite /M_rec; left; exists m; split; [apply ineq | rewrite /M_rec b].
+  by rewrite /M_rec; left; exists m; split; [apply ineq | rewrite /M_rec b].
 have [ | k val]//:= prp n.
 case E: (mf (listf (map phi (init_seg k))) q' <= k).
-	by left; exists k; split =>//=; rewrite val /M_step /psiF/= size_map size_iseg E.
+  by left; exists k; split =>//=; rewrite val /M_step /psiF/= size_map size_iseg E.
 right => m; rewrite leq_eqVlt; case/orP => [/eqP -> /= | le]; last exact/prp.
 rewrite val/M_step/psiF/= size_map size_iseg E.
 exists (mf (listf [seq phi i | i <- init_seg k]) q').
 f_equal; rewrite -map_cat; f_equal; case: k prp E val => [prp E val | k prp E val].
-	by rewrite cats0; case: (mf (listf [seq phi i | i <- init_seg 0]) q') E => // h E; rewrite iseg_seg.
+  by rewrite cats0; case: (mf (listf [seq phi i | i <- init_seg 0]) q') E => // h E; rewrite iseg_seg.
 by rewrite iseg_cat_seg // ltnNge E.
 Qed.
-
-Definition mod_mod mf (phi: B):= continuity_modulus (F2MF mf) phi (fun (q': Q') => init_seg (mf phi q')).
 
 Lemma MpsiF_spec (F: B ->> B') phi: phi \from dom F ->
 	(forall n, listf (map phi (init_seg n)) \from dom F) ->
@@ -285,19 +280,19 @@ Proof.
 move => phifd listfdom listfcoin listfmod mod icf Fphi FphiFphi q'.
 pose phin n := (listf (map phi (init_seg n))).
 have FFprop: forall n, mf (phin n) q' <= n -> FF (phin n) q' = Fphi q' => [n ineq | ].
-	have [ | a' crt]:= mod (phin n) _ q'; first exact/listfdom; have [Fphik FphikFphik]:= listfdom n.
-	rewrite [RHS](crt phi) => //; first by rewrite (crt (phin n)) //; apply/icf/FphikFphik.
-	exact/coin_spec/coin_subl/listfcoin/iseg_subl/ineq.
-elim: {2}(mf phi q') (leqnn (mf phi q')) => [ | n ih]; last first.
-	case: (psiF_spec phi q' n) => [[k [nlk eq]] | prp].
-		by exists n.+1; rewrite /M/=eq; f_equal; exact/FFprop/nlk.
-	rewrite leq_eqVlt => /orP [/eqP eq| ineq]; last exact/ih.
-	have [ | k val]//:= prp n; exists n.+1; rewrite /M/=val/M_step/psiF/=size_map size_iseg.
-	suff bnd: mf (listf [seq phi i | i <- init_seg k]) q' <= k by rewrite bnd; f_equal; apply/FFprop.
-	by apply/leq_trans; first apply/(listfmod q');
-		rewrite eq; have:= psiF_size val; rewrite size_map size_iseg.
-move => ineq; exists 0; rewrite /M/psiF/=/M_step /=.
-have eq': mf (listf nil) q' <= 0 by apply/leq_trans/ineq/leq_trans/(listfmod q' 0).
-by rewrite eq'; f_equal; apply/(FFprop 0).
+- have [ | a' crt]:= mod (phin n) _ q'; first exact/listfdom; have [Fphik FphikFphik]:= listfdom n.
+  rewrite [RHS](crt phi) => //; first by rewrite (crt (phin n)) //; apply/icf/FphikFphik.
+  exact/coin_spec/coin_subl/listfcoin/iseg_subl/ineq.
+elim: {2}(mf phi q') (leqnn (mf phi q')) => [ineq | n ih].
+- exists 0; rewrite /M/psiF/=/M_step /=.
+  have eq': mf (listf nil) q' <= 0 by apply/leq_trans/ineq/leq_trans/(listfmod q' 0).
+  by rewrite eq'; f_equal; apply/(FFprop 0).
+case: (psiF_spec phi q' n) => [[k [nlk eq]] | prp].
+  by exists n.+1; rewrite /M/=eq; f_equal; exact/FFprop/nlk.
+rewrite leq_eqVlt => /orP [/eqP eq| ineq]; last exact/ih.
+have [ | k val]//:= prp n; exists n.+1; rewrite /M/=val/M_step/psiF/=size_map size_iseg.
+suff bnd: mf (listf [seq phi i | i <- init_seg k]) q' <= k by rewrite bnd; f_equal; apply/FFprop.
+by apply/leq_trans; first apply/(listfmod q');
+rewrite eq; have:= psiF_size val; rewrite size_map size_iseg.
 Qed.
 End psiF.
